proofs/fstar/extraction/Sandwich.Tunnel.Rec_bundle_522409734.fst
@@ -1,4 +1,4 @@
-module Sandwich.Tunnel.Rec_bundle_818341900
+module Sandwich.Tunnel.Rec_bundle_522409734
 #set-options "--fuel 0 --ifuel 1 --z3rlimit 15"
 open Core
 open FStar.Mul
@@ -6,19 +6,16 @@ open FStar.Mul
 let _ =
   (* This module has implicit dependencies, here we make them explicit. *)
   (* The implicit dependencies arise from typeclasses instances. *)
-  let open Sandwich in
   let open Sandwich.Error in
   let open Sandwich.Error.Code in
   let open Sandwich.Implementation.Openssl3_impl.Tunnel.X509_verify_param in
-  let open Sandwich.Tunnel.Context in
   let open Sandwich.Tunnel.Tls in
+  let open Alloc.Vec in
+  let open Core.Iter.Traits.Collect in
   ()
 
 /// Convenient wrapper around a `SSL_CTX`.
 type t_SslContext = | SslContext : Core.Ptr.Non_null.t_NonNull Openssl3.t_ssl_ctx_st -> t_SslContext
-
-/// Wrapper of the OpenSSL SSL object.
-type t_Ssl = | Ssl : Core.Ptr.Non_null.t_NonNull Openssl3.t_ssl_st -> t_Ssl
 
 /// Mode for a [`Context`].
 /// A [`Context`] is either a context for client-side applications or
@@ -34,24 +31,6 @@ type t_Context116464909 = {
   f_security_requirements:Sandwich.Tunnel.Tls.t_TunnelSecurityRequirements;
   f_mode:t_Mode
 }
-
-[@@ FStar.Tactics.Typeclasses.tcinstance]
-let impl_1: Core.Borrow.t_Borrow t_Context116464909 Sandwich.Tunnel.Tls.t_TunnelSecurityRequirements =
-  {
-    f_borrow_pre = (fun (self: t_Context116464909) -> true);
-    f_borrow_post
-    =
-    (fun (self: t_Context116464909) (out: Sandwich.Tunnel.Tls.t_TunnelSecurityRequirements) -> true);
-    f_borrow = fun (self: t_Context116464909) -> self.f_security_requirements
-  }
-
-/// Returns the security requirements of the context.
-let security_requirements (self: t_Context116464909)
-    : Sandwich.Tunnel.Tls.t_TunnelSecurityRequirements =
-  Core.Borrow.f_borrow #t_Context116464909
-    #Sandwich.Tunnel.Tls.t_TunnelSecurityRequirements
-    #FStar.Tactics.Typeclasses.solve
-    self
 
 /// A Sandwich context.
 type t_Context665818913 = | Context665818913_OpenSSL3 : t_Context116464909 -> t_Context665818913
@@ -86,13 +65,6 @@ let get_verify_mode_from_mode_and_x509_verifier
     if mode =. (Mode_Client <: t_Mode)
     then Sandwich.Tunnel.Tls.VerifyMode_Peer <: Sandwich.Tunnel.Tls.t_VerifyMode
     else Sandwich.Tunnel.Tls.VerifyMode_Mutual <: Sandwich.Tunnel.Tls.t_VerifyMode
-
-/// Instantiates a new SSL object.
-assume
-val new_ssl': self: t_Context116464909
-  -> Core.Result.t_Result (Sandwich.Support.Pimpl.t_Pimpl Openssl3.t_ssl_st) Sandwich.Error.t_Error
-
-let new_ssl = new_ssl'
 
 /// Configures TLS 1.2.
 assume
@@ -143,7 +115,8 @@ val set_alpn_protocols':
     protocols: impl_995885649_
   -> Core.Result.t_Result Prims.unit Sandwich.Error.t_Error
 
-let set_alpn_protocols = set_alpn_protocols'
+let set_alpn_protocols #v_S #impl_995885649_ {| i6: Core.Convert.t_AsRef v_S string |} {| i61: Core.Iter.Traits.Collect.t_IntoIterator impl_995885649_ |}= 
+  set_alpn_protocols' #v_S #impl_995885649_ #i6 #i61
 
 /// Sets the default parameters for a SSL context.
 assume
@@ -190,39 +163,22 @@ val new_ssl_context': ctx: Sandwich.t_Context -> mode: t_Mode
 
 let new_ssl_context = new_ssl_context'
 
-/// Creates a new Sandwich BIO and attach it to the SSL object.
-assume
-val create_and_attach_bio': self: t_Ssl -> Core.Result.t_Result Prims.unit Sandwich.Error.t_Error
-
-let create_and_attach_bio = create_and_attach_bio'
-
-/// Sets the server name indication (SNI).
-assume
-val set_server_name_indication':
-    #impl_488124255_: Type0 ->
-    {| i9: Core.Convert.t_AsRef impl_488124255_ string |} ->
-    self: t_Ssl ->
-    sni: impl_488124255_
-  -> Core.Result.t_Result Prims.unit Sandwich.Error.t_Error
-
-let set_server_name_indication = set_server_name_indication'
-
 /// Returns the execution mode (Client or Server) and the tls options (`TLSOptions`).
 let configuration_get_mode_and_options
       (configuration: Sandwich_api_proto.Configuration.t_Configuration)
     : Core.Result.t_Result (t_Mode & Sandwich_api_proto.Tls.t_TLSOptions) Sandwich.Error.t_Error =
   Core.Option.impl__ok_or #(t_Mode & Sandwich_api_proto.Tls.t_TLSOptions)
     #Sandwich.Error.t_Error
-    (Core.Option.impl__and_then #Sandwich_api_proto.Configuration.Configuration.t_Opts
+    (Core.Option.impl__and_then #Sandwich_api_proto.Configuration.t_Opts
         #(t_Mode & Sandwich_api_proto.Tls.t_TLSOptions)
-        (Core.Option.impl__as_ref #Sandwich_api_proto.Configuration.Configuration.t_Opts
+        (Core.Option.impl__as_ref #Sandwich_api_proto.Configuration.t_Opts
             configuration.Sandwich_api_proto.Configuration.f_opts
           <:
-          Core.Option.t_Option Sandwich_api_proto.Configuration.Configuration.t_Opts)
+          Core.Option.t_Option Sandwich_api_proto.Configuration.t_Opts)
         (fun opts ->
-            let opts:Sandwich_api_proto.Configuration.Configuration.t_Opts = opts in
+            let opts:Sandwich_api_proto.Configuration.t_Opts = opts in
             match opts with
-            | Sandwich_api_proto.Configuration.Configuration.Opts_Client opt ->
+            | Sandwich_api_proto.Configuration.Opts_Client opt ->
               Core.Option.impl__map #Sandwich_api_proto.Tls.t_TLSOptions
                 #(t_Mode & Sandwich_api_proto.Tls.t_TLSOptions)
                 (Core.Option.impl__and_then #Sandwich_api_proto.Tls.t_TLSClientOptions
@@ -262,7 +218,7 @@ let configuration_get_mode_and_options
                     (Mode_Client <: t_Mode), tls <: (t_Mode & Sandwich_api_proto.Tls.t_TLSOptions))
               <:
               Core.Option.t_Option (t_Mode & Sandwich_api_proto.Tls.t_TLSOptions)
-            | Sandwich_api_proto.Configuration.Configuration.Opts_Server opt ->
+            | Sandwich_api_proto.Configuration.Opts_Server opt ->
               Core.Option.impl__map #Sandwich_api_proto.Tls.t_TLSOptions
                 #(t_Mode & Sandwich_api_proto.Tls.t_TLSOptions)
                 (Core.Option.impl__and_then #Sandwich_api_proto.Tls.t_TLSServerOptions
@@ -420,18 +376,13 @@ let try_from
       (ctx: Sandwich.t_Context)
       (configuration: Sandwich_api_proto.Configuration.t_Configuration)
     : Core.Result.t_Result t_Context116464909 Sandwich.Error.t_Error =
-  let lib_ctx:Sandwich.Implementation.Openssl3_impl.t_LibCtx =
-    Core.Borrow.f_borrow #Sandwich.t_Context
-      #Sandwich.Implementation.Openssl3_impl.t_LibCtx
-      #FStar.Tactics.Typeclasses.solve
-      ctx
-  in
+  let lib_ctx:Sandwich.Implementation.Openssl3_impl.t_LibCtx = ctx.Sandwich.f_ossl3_lib_ctx in
   match configuration_get_mode_and_options configuration with
   | Core.Result.Result_Ok (mode, tls_options) ->
     (match new_ssl_context ctx mode with
       | Core.Result.Result_Ok ssl_ctx ->
         let ssl_ctx_wrapped:t_SslContext =
-          t_SslContext (Sandwich.Support.Pimpl.impl_2__as_nonnull #Openssl3.t_ssl_ctx_st ssl_ctx)
+          SslContext (Sandwich.Support.Pimpl.impl_2__as_nonnull #Openssl3.t_ssl_ctx_st ssl_ctx)
           <:
           t_SslContext
         in
@@ -459,17 +410,9 @@ let try_from
                           | Core.Result.Result_Ok _ ->
                             (match
                                 set_alpn_protocols #Alloc.String.t_String
-                                  #(Core.Slice.Iter.t_Iter Alloc.String.t_String)
+                                  #(Alloc.Vec.t_Vec Alloc.String.t_String Alloc.Alloc.t_Global)
                                   ssl_ctx_wrapped
-                                  (Core.Slice.impl__iter #Alloc.String.t_String
-                                      (Core.Ops.Deref.f_deref #(Alloc.Vec.t_Vec
-                                              Alloc.String.t_String Alloc.Alloc.t_Global)
-                                          #FStar.Tactics.Typeclasses.solve
-                                          tls_options.Sandwich_api_proto.Tls.f_alpn_protocols
-                                        <:
-                                        t_Slice Alloc.String.t_String)
-                                    <:
-                                    Core.Slice.Iter.t_Iter Alloc.String.t_String)
+                                  tls_options.Sandwich_api_proto.Tls.f_alpn_protocols
                               with
                               | Core.Result.Result_Ok _ ->
                                 (match
@@ -542,7 +485,18 @@ let try_from
                                                             (Core.Option.impl__map #Sandwich_api_proto.Verifiers.t_X509Verifier
                                                                 #Sandwich.Tunnel.Tls.t_TunnelSecurityRequirements
                                                                 x509_verifier
-                                                                Core.Convert.From.from
+                                                                (fun x ->
+                                                                    let x:Sandwich_api_proto.Verifiers.t_X509Verifier
+                                                                    =
+                                                                      x
+                                                                    in
+                                                                    Core.Convert.f_from #Sandwich.Tunnel.Tls.t_TunnelSecurityRequirements
+                                                                      #Sandwich_api_proto.Verifiers.t_X509Verifier
+                                                                      #FStar.Tactics.Typeclasses.solve
+                                                                      x
+                                                                    <:
+                                                                    Sandwich.Tunnel.Tls.t_TunnelSecurityRequirements
+                                                                )
                                                               <:
                                                               Core.Option.t_Option
                                                               Sandwich.Tunnel.Tls.t_TunnelSecurityRequirements
@@ -626,209 +580,6 @@ let hax_try_from
       (configuration: Sandwich_api_proto.Configuration.t_Configuration)
     : Core.Result.t_Result t_Context116464909 Sandwich.Error.t_Error = try_from ctx configuration
 
-/// Sets the required Subject Alternative Names (SAN) specified in the [`pb_api::TunnelVerifier`]
-/// object.
-let set_subject_alternative_names
-      (self: t_Ssl)
-      (tunnel_verifier: Core.Option.t_Option Sandwich_api_proto.Verifiers.t_TunnelVerifier)
-    : Core.Result.t_Result Prims.unit Sandwich.Error.t_Error =
-  match
-    Core.Option.impl__and_then #Sandwich_api_proto.Verifiers.t_TunnelVerifier
-      #Sandwich_api_proto.Verifiers.Tunnel_verifier.t_Verifier
-      tunnel_verifier
-      (fun tv ->
-          let tv:Sandwich_api_proto.Verifiers.t_TunnelVerifier = tv in
-          Core.Option.impl__as_ref #Sandwich_api_proto.Verifiers.Tunnel_verifier.t_Verifier
-            tv.Sandwich_api_proto.Verifiers.f_verifier
-          <:
-          Core.Option.t_Option Sandwich_api_proto.Verifiers.Tunnel_verifier.t_Verifier)
-  with
-  | Core.Option.Option_Some
-    (Sandwich_api_proto.Verifiers.Tunnel_verifier.Verifier_SanVerifier san_verifier) ->
-    (match
-        Core.Convert.f_try_from #Sandwich.Implementation.Openssl3_impl.Tunnel.X509_verify_param.t_X509VerifyParam
-          #(Core.Ptr.Non_null.t_NonNull Openssl3.t_ssl_st)
-          #FStar.Tactics.Typeclasses.solve
-          self._0
-      with
-      | Core.Result.Result_Ok x509_verify_param ->
-        (match
-            Rust_primitives.Hax.f_fold_return (Core.Iter.Traits.Collect.f_into_iter #(Core.Slice.Iter.t_Iter
-                    Sandwich_api_proto.Verifiers.t_SANMatcher)
-                  #FStar.Tactics.Typeclasses.solve
-                  (Core.Slice.impl__iter #Sandwich_api_proto.Verifiers.t_SANMatcher
-                      (Core.Ops.Deref.f_deref #(Alloc.Vec.t_Vec
-                              Sandwich_api_proto.Verifiers.t_SANMatcher Alloc.Alloc.t_Global)
-                          #FStar.Tactics.Typeclasses.solve
-                          san_verifier.Sandwich_api_proto.Verifiers.f_alt_names
-                        <:
-                        t_Slice Sandwich_api_proto.Verifiers.t_SANMatcher)
-                    <:
-                    Core.Slice.Iter.t_Iter Sandwich_api_proto.Verifiers.t_SANMatcher)
-                <:
-                Core.Slice.Iter.t_Iter Sandwich_api_proto.Verifiers.t_SANMatcher)
-              ()
-              (fun temp_0_ san ->
-                  let _:Prims.unit = temp_0_ in
-                  let san:Sandwich_api_proto.Verifiers.t_SANMatcher = san in
-                  match
-                    Core.Option.impl__as_ref #Sandwich_api_proto.Verifiers.Sanmatcher.t_San
-                      san.Sandwich_api_proto.Verifiers.f_san
-                    <:
-                    Core.Option.t_Option Sandwich_api_proto.Verifiers.Sanmatcher.t_San
-                  with
-                  | Core.Option.Option_Some san ->
-                    (match
-                        Sandwich.Implementation.Openssl3_impl.Tunnel.X509_verify_param.impl_4__add_san
-                          x509_verify_param
-                          san
-                        <:
-                        Core.Result.t_Result Prims.unit Sandwich.Error.t_Error
-                      with
-                      | Core.Result.Result_Ok _ ->
-                        Core.Ops.Control_flow.ControlFlow_Continue ()
-                        <:
-                        Core.Ops.Control_flow.t_ControlFlow
-                          (Core.Ops.Control_flow.t_ControlFlow
-                              (Core.Result.t_Result Prims.unit Sandwich.Error.t_Error)
-                              (Prims.unit & Prims.unit)) Prims.unit
-                      | Core.Result.Result_Err err ->
-                        Core.Ops.Control_flow.ControlFlow_Break
-                        (Core.Ops.Control_flow.ControlFlow_Break
-                          (Core.Result.Result_Err err
-                            <:
-                            Core.Result.t_Result Prims.unit Sandwich.Error.t_Error)
-                          <:
-                          Core.Ops.Control_flow.t_ControlFlow
-                            (Core.Result.t_Result Prims.unit Sandwich.Error.t_Error)
-                            (Prims.unit & Prims.unit))
-                        <:
-                        Core.Ops.Control_flow.t_ControlFlow
-                          (Core.Ops.Control_flow.t_ControlFlow
-                              (Core.Result.t_Result Prims.unit Sandwich.Error.t_Error)
-                              (Prims.unit & Prims.unit)) Prims.unit)
-                  | _ ->
-                    Core.Ops.Control_flow.ControlFlow_Break
-                    (Core.Ops.Control_flow.ControlFlow_Break
-                      (Core.Result.Result_Err
-                        (Core.Convert.f_into #(Sandwich_proto.Errors.t_TunnelError & string)
-                            #Sandwich.Error.t_Error
-                            #FStar.Tactics.Typeclasses.solve
-                            ((Sandwich_proto.Errors.TunnelError_TUNNELERROR_VERIFIER
-                                <:
-                                Sandwich_proto.Errors.t_TunnelError),
-                              "empty SANMatcher"
-                              <:
-                              (Sandwich_proto.Errors.t_TunnelError & string))
-                          <:
-                          Sandwich.Error.t_Error)
-                        <:
-                        Core.Result.t_Result Prims.unit Sandwich.Error.t_Error)
-                      <:
-                      Core.Ops.Control_flow.t_ControlFlow
-                        (Core.Result.t_Result Prims.unit Sandwich.Error.t_Error)
-                        (Prims.unit & Prims.unit))
-                    <:
-                    Core.Ops.Control_flow.t_ControlFlow
-                      (Core.Ops.Control_flow.t_ControlFlow
-                          (Core.Result.t_Result Prims.unit Sandwich.Error.t_Error)
-                          (Prims.unit & Prims.unit)) Prims.unit)
-          with
-          | Core.Ops.Control_flow.ControlFlow_Break ret -> ret
-          | Core.Ops.Control_flow.ControlFlow_Continue _ ->
-            Core.Result.Result_Ok (() <: Prims.unit)
-            <:
-            Core.Result.t_Result Prims.unit Sandwich.Error.t_Error)
-      | Core.Result.Result_Err err ->
-        Core.Result.Result_Err err <: Core.Result.t_Result Prims.unit Sandwich.Error.t_Error)
-  | _ ->
-    Core.Result.Result_Ok (() <: Prims.unit)
-    <:
-    Core.Result.t_Result Prims.unit Sandwich.Error.t_Error
-
-/// Verifies the tunnel configuration against the security requirements that come
-/// from the context.
-let verify_tunnel_verifier
-      (tunnel_verifier: Core.Option.t_Option Sandwich_api_proto.Verifiers.t_TunnelVerifier)
-      (security_requirements: Sandwich.Tunnel.Tls.t_TunnelSecurityRequirements)
-    : Core.Result.t_Result Prims.unit Sandwich.Error.t_Error =
-  match tunnel_verifier with
-  | Core.Option.Option_Some tunnel_verifier ->
-    Sandwich.Tunnel.Tls.f_run_sanitizer_checks #Sandwich.Tunnel.Tls.t_TunnelSecurityRequirements
-      #Sandwich_api_proto.Verifiers.t_TunnelVerifier
-      #FStar.Tactics.Typeclasses.solve
-      security_requirements
-      tunnel_verifier
-  | _ ->
-    Core.Result.Result_Err
-    (Core.Convert.f_into #(Sandwich_proto.Errors.t_TunnelError & string)
-        #Sandwich.Error.t_Error
-        #FStar.Tactics.Typeclasses.solve
-        ((Sandwich_proto.Errors.TunnelError_TUNNELERROR_VERIFIER
-            <:
-            Sandwich_proto.Errors.t_TunnelError),
-          "empty verifier"
-          <:
-          (Sandwich_proto.Errors.t_TunnelError & string)))
-    <:
-    Core.Result.t_Result Prims.unit Sandwich.Error.t_Error
-
-/// Prepares a tunnel structure.
-let prepare_ssl (self: t_TunnelBuilder)
-    : Core.Result.t_Result (Sandwich.Support.Pimpl.t_Pimpl Openssl3.t_ssl_st) Sandwich.Error.t_Error =
-  let tunnel_verifier:Core.Option.t_Option Sandwich_api_proto.Verifiers.t_TunnelVerifier =
-    Protobuf.Message_field.impl__as_ref #Sandwich_api_proto.Verifiers.t_TunnelVerifier
-      self.f_configuration.Sandwich_api_proto.Tunnel.f_verifier
-  in
-  let security_requirements:Sandwich.Tunnel.Tls.t_TunnelSecurityRequirements =
-    security_requirements self.f_ssl_ctx
-  in
-  match verify_tunnel_verifier tunnel_verifier security_requirements with
-  | Core.Result.Result_Ok _ ->
-    (match new_ssl self.f_ssl_ctx with
-      | Core.Result.Result_Ok ssl ->
-        let ssl_wrapped:t_Ssl =
-          t_Ssl (Sandwich.Support.Pimpl.impl_2__as_nonnull #Openssl3.t_ssl_st ssl) <: t_Ssl
-        in
-        (match set_subject_alternative_names ssl_wrapped tunnel_verifier with
-          | Core.Result.Result_Ok _ ->
-            (match
-                set_server_name_indication #Alloc.String.t_String
-                  ssl_wrapped
-                  self.f_configuration.Sandwich_api_proto.Tunnel.f_server_name_indication
-              with
-              | Core.Result.Result_Ok _ ->
-                (match create_and_attach_bio ssl_wrapped with
-                  | Core.Result.Result_Ok _ ->
-                    Core.Result.Result_Ok ssl
-                    <:
-                    Core.Result.t_Result (Sandwich.Support.Pimpl.t_Pimpl Openssl3.t_ssl_st)
-                      Sandwich.Error.t_Error
-                  | Core.Result.Result_Err err ->
-                    Core.Result.Result_Err err
-                    <:
-                    Core.Result.t_Result (Sandwich.Support.Pimpl.t_Pimpl Openssl3.t_ssl_st)
-                      Sandwich.Error.t_Error)
-              | Core.Result.Result_Err err ->
-                Core.Result.Result_Err err
-                <:
-                Core.Result.t_Result (Sandwich.Support.Pimpl.t_Pimpl Openssl3.t_ssl_st)
-                  Sandwich.Error.t_Error)
-          | Core.Result.Result_Err err ->
-            Core.Result.Result_Err err
-            <:
-            Core.Result.t_Result (Sandwich.Support.Pimpl.t_Pimpl Openssl3.t_ssl_st)
-              Sandwich.Error.t_Error)
-      | Core.Result.Result_Err err ->
-        Core.Result.Result_Err err
-        <:
-        Core.Result.t_Result (Sandwich.Support.Pimpl.t_Pimpl Openssl3.t_ssl_st)
-          Sandwich.Error.t_Error)
-  | Core.Result.Result_Err err ->
-    Core.Result.Result_Err err
-    <:
-    Core.Result.t_Result (Sandwich.Support.Pimpl.t_Pimpl Openssl3.t_ssl_st) Sandwich.Error.t_Error
-
 /// A tunnel, wrapper around a SSL object.
 type t_Tunnel364847772 = {
   f__ssl_ctx:t_Context116464909;
@@ -838,109 +589,14 @@ type t_Tunnel364847772 = {
   f_state:Sandwich_proto.Tunnel.t_State
 }
 
-/// Attaches the security requirements structure to the `SSL` object
-/// through `ex_data`.
-assume
-val attach_security_requirements': self: Core.Pin.t_Pin t_Tunnel364847772
-  -> Core.Result.t_Result Prims.unit Sandwich.Error.t_Error
-
-let attach_security_requirements = attach_security_requirements'
-
-/// Attaches itself to the current BIO.
-assume
-val attach_to_bio': self: Core.Pin.t_Pin t_Tunnel364847772
-  -> Core.Result.t_Result Prims.unit Sandwich.Error.t_Error
-
-let attach_to_bio = attach_to_bio'
-
-/// A tunnel.
-type t_Tunnel70284935 =
-  | Tunnel70284935_OpenSSL3 :
-      Core.Pin.t_Pin (Alloc.Boxed.t_Box t_Tunnel364847772 Alloc.Alloc.t_Global)
-    -> t_Tunnel70284935
-
 /// Builds a tunnel.
-let build (self: t_TunnelBuilder)
-    : Core.Result.t_Result
+assume
+val build': self: t_TunnelBuilder
+  -> Core.Result.t_Result
       (Core.Pin.t_Pin (Alloc.Boxed.t_Box t_Tunnel364847772 Alloc.Alloc.t_Global))
-      (Sandwich.Error.t_Error & Sandwich.Tunnel.Io.t_BoxedIO) =
-  match prepare_ssl self with
-  | Core.Result.Result_Ok ssl ->
-    let ssl:Sandwich.Support.Pimpl.t_Pimpl Openssl3.t_ssl_st = ssl in
-    let tun:Core.Pin.t_Pin (Alloc.Boxed.t_Box t_Tunnel364847772 Alloc.Alloc.t_Global) =
-      Alloc.Boxed.impl__pin #t_Tunnel364847772
-        ({
-            f__ssl_ctx = self.f_ssl_ctx;
-            f_ssl = ssl;
-            f_io = self.f_io;
-            f_security_requirements
-            =
-            Core.Clone.f_clone #Sandwich.Tunnel.Tls.t_TunnelSecurityRequirements
-              #FStar.Tactics.Typeclasses.solve
-              (security_requirements self.f_ssl_ctx
-                <:
-                Sandwich.Tunnel.Tls.t_TunnelSecurityRequirements)
-            <:
-            Sandwich.Tunnel.Tls.t_TunnelSecurityRequirements;
-            f_state
-            =
-            Sandwich_proto.Tunnel.State_STATE_NOT_CONNECTED <: Sandwich_proto.Tunnel.t_State
-          }
-          <:
-          t_Tunnel364847772)
-    in
-    (match
-        attach_security_requirements (Core.Pin.impl_6__as_ref #(Alloc.Boxed.t_Box t_Tunnel364847772
-                  Alloc.Alloc.t_Global)
-              tun
-            <:
-            Core.Pin.t_Pin t_Tunnel364847772)
-      with
-      | Core.Result.Result_Err e ->
-        Core.Result.Result_Err
-        (e,
-          (Core.Pin.impl_8__into_inner_unchecked #(Alloc.Boxed.t_Box t_Tunnel364847772
-                  Alloc.Alloc.t_Global)
-              tun)
-            .f_io
-          <:
-          (Sandwich.Error.t_Error & Sandwich.Tunnel.Io.t_BoxedIO))
-        <:
-        Core.Result.t_Result
-          (Core.Pin.t_Pin (Alloc.Boxed.t_Box t_Tunnel364847772 Alloc.Alloc.t_Global))
-          (Sandwich.Error.t_Error & Sandwich.Tunnel.Io.t_BoxedIO)
-      | _ ->
-        match
-          attach_to_bio (Core.Pin.impl_6__as_ref #(Alloc.Boxed.t_Box t_Tunnel364847772
-                    Alloc.Alloc.t_Global)
-                tun
-              <:
-              Core.Pin.t_Pin t_Tunnel364847772)
-        with
-        | Core.Result.Result_Err e ->
-          Core.Result.Result_Err
-          (e,
-            (Core.Pin.impl_8__into_inner_unchecked #(Alloc.Boxed.t_Box t_Tunnel364847772
-                    Alloc.Alloc.t_Global)
-                tun)
-              .f_io
-            <:
-            (Sandwich.Error.t_Error & Sandwich.Tunnel.Io.t_BoxedIO))
-          <:
-          Core.Result.t_Result
-            (Core.Pin.t_Pin (Alloc.Boxed.t_Box t_Tunnel364847772 Alloc.Alloc.t_Global))
-            (Sandwich.Error.t_Error & Sandwich.Tunnel.Io.t_BoxedIO)
-        | _ ->
-          Core.Result.Result_Ok tun
-          <:
-          Core.Result.t_Result
-            (Core.Pin.t_Pin (Alloc.Boxed.t_Box t_Tunnel364847772 Alloc.Alloc.t_Global))
-            (Sandwich.Error.t_Error & Sandwich.Tunnel.Io.t_BoxedIO))
-  | Core.Result.Result_Err e ->
-    Core.Result.Result_Err (e, self.f_io <: (Sandwich.Error.t_Error & Sandwich.Tunnel.Io.t_BoxedIO))
-    <:
-    Core.Result.t_Result (Core.Pin.t_Pin (Alloc.Boxed.t_Box t_Tunnel364847772 Alloc.Alloc.t_Global))
       (Sandwich.Error.t_Error & Sandwich.Tunnel.Io.t_BoxedIO)
+
+let build = build'
 
 /// Creates a new tunnel.
 let new_tunnel474967037
@@ -952,6 +608,12 @@ let new_tunnel474967037
       (Sandwich.Error.t_Error & Sandwich.Tunnel.Io.t_BoxedIO) =
   build ({ f_ssl_ctx = self; f_io = io; f_configuration = configuration } <: t_TunnelBuilder)
 
+/// A tunnel.
+type t_Tunnel70284935 =
+  | Tunnel70284935_OpenSSL3 :
+      Core.Pin.t_Pin (Alloc.Boxed.t_Box t_Tunnel364847772 Alloc.Alloc.t_Global)
+    -> t_Tunnel70284935
+
 /// Creates a new tunnel from an I/O interface. See [`IO`] from [`crate::io`] module.
 /// The I/O interface must outlive the tunnel, as the tunnel makes use
 /// of it to send and receive data.
@@ -962,10 +624,10 @@ let new_tunnel499954878
       (configuration: Sandwich_api_proto.Tunnel.t_TunnelConfiguration)
     : Core.Result.t_Result t_Tunnel70284935 (Sandwich.Error.t_Error & Sandwich.Tunnel.Io.t_BoxedIO) =
   match self with
-  | (Context665818913_OpenSSL3 c: t_Context665818913) ->
+  | (Context665818913_OpenSSL3 c(*: t_Context665818913*)) ->
     match new_tunnel474967037 c io configuration with
-    | Core.Result.Result_Ok hoist5 ->
-      Core.Result.Result_Ok (Tunnel70284935_OpenSSL3 hoist5 <: t_Tunnel70284935)
+    | Core.Result.Result_Ok hoist1 ->
+      Core.Result.Result_Ok (Tunnel70284935_OpenSSL3 hoist1 <: t_Tunnel70284935)
       <:
       Core.Result.t_Result t_Tunnel70284935 (Sandwich.Error.t_Error & Sandwich.Tunnel.Io.t_BoxedIO)
     | Core.Result.Result_Err err ->
