proofs/fstar/extraction/Sandwich.fst
@@ -6,13 +6,3 @@ open FStar.Mul
 /// Top-level context.
 /// This context is used to create tunnel contexts.
 type t_Context = { f_ossl3_lib_ctx:Sandwich.Implementation.Openssl3_impl.t_LibCtx }
-
-[@@ FStar.Tactics.Typeclasses.tcinstance]
-let impl_2: Core.Borrow.t_Borrow t_Context Sandwich.Implementation.Openssl3_impl.t_LibCtx =
-  {
-    f_borrow_pre = (fun (self: t_Context) -> true);
-    f_borrow_post
-    =
-    (fun (self: t_Context) (out: Sandwich.Implementation.Openssl3_impl.t_LibCtx) -> true);
-    f_borrow = fun (self: t_Context) -> self.f_ossl3_lib_ctx
-  }
