proofs/fstar/extraction/Sandwich.Implementation.Openssl3_impl.Tunnel.Ssl.fst
@@ -3,30 +3,12 @@ module Sandwich.Implementation.Openssl3_impl.Tunnel.Ssl
 open Core
 open FStar.Mul
 
-include Sandwich.Tunnel.Rec_bundle_818341900 {t_Ssl as t_Ssl}
+include Sandwich.Tunnel.Rec_bundle_522409734 {t_TunnelBuilder as t_TunnelBuilder}
 
-include Sandwich.Tunnel.Rec_bundle_818341900 {_0 as _0}
+include Sandwich.Tunnel.Rec_bundle_522409734 {f_ssl_ctx as f_ssl_ctx}
 
-include Sandwich.Tunnel.Rec_bundle_818341900 {t_TunnelBuilder as t_TunnelBuilder}
+include Sandwich.Tunnel.Rec_bundle_522409734 {f_io as f_io}
 
-include Sandwich.Tunnel.Rec_bundle_818341900 {f_ssl_ctx as f_ssl_ctx}
+include Sandwich.Tunnel.Rec_bundle_522409734 {f_configuration as f_configuration}
 
-include Sandwich.Tunnel.Rec_bundle_818341900 {f_io as f_io}
-
-include Sandwich.Tunnel.Rec_bundle_818341900 {f_configuration as f_configuration}
-
-include Sandwich.Tunnel.Rec_bundle_818341900 {create_and_attach_bio as impl__Ssl__create_and_attach_bio}
-
-include Sandwich.Tunnel.Rec_bundle_818341900 {set_server_name_indication as impl__Ssl__set_server_name_indication}
-
-include Sandwich.Tunnel.Rec_bundle_818341900 {set_subject_alternative_names as impl__Ssl__set_subject_alternative_names}
-
-include Sandwich.Tunnel.Rec_bundle_818341900 {verify_tunnel_verifier as verify_tunnel_verifier}
-
-include Sandwich.Tunnel.Rec_bundle_818341900 {prepare_ssl as impl_5__prepare_ssl}
-
-include Sandwich.Tunnel.Rec_bundle_818341900 {attach_security_requirements as impl_6__attach_security_requirements}
-
-include Sandwich.Tunnel.Rec_bundle_818341900 {attach_to_bio as impl_6__attach_to_bio}
-
-include Sandwich.Tunnel.Rec_bundle_818341900 {build as impl_5__build}
+include Sandwich.Tunnel.Rec_bundle_522409734 {build as impl_5__build}
