proofs/fstar/extraction/Sandwich.Tunnel.Io.fst
@@ -1,0 +1,10 @@
+module Sandwich.Tunnel.Io
+#set-options "--fuel 0 --ifuel 1 --z3rlimit 15"
+open Core
+open FStar.Mul
+
+/// BoxedIO
+assume
+val t_BoxedIO': Type0
+
+let t_BoxedIO = t_BoxedIO'
