proofs/fstar/extraction/Sandwich.Tunnel.Tls.Support.fst
@@ -3,8 +3,8 @@ module Sandwich.Tunnel.Tls.Support
 open Core
 open FStar.Mul
 
-include Sandwich.Tunnel.Rec_bundle_818341900 {configuration_get_mode_and_options as configuration_get_mode_and_options}
+include Sandwich.Tunnel.Rec_bundle_522409734 {configuration_get_mode_and_options as configuration_get_mode_and_options}
 
-include Sandwich.Tunnel.Rec_bundle_818341900 {tls_options_get_x509_verifier as tls_options_get_x509_verifier}
+include Sandwich.Tunnel.Rec_bundle_522409734 {tls_options_get_x509_verifier as tls_options_get_x509_verifier}
 
-include Sandwich.Tunnel.Rec_bundle_818341900 {x509_verifier_verify_emptiness as x509_verifier_verify_emptiness}
+include Sandwich.Tunnel.Rec_bundle_522409734 {x509_verifier_verify_emptiness as x509_verifier_verify_emptiness}
