rust_vendor/sandwich-api-proto/proofs/fstar/Sandwich_api_proto.Configuration.Configuration.fst
@@ -1,0 +1,17 @@
+module Sandwich_api_proto.Configuration.Configuration
+#set-options "--fuel 0 --ifuel 1 --z3rlimit 15"
+open Core
+open FStar.Mul
+(*
+include Sandwich_api_proto.Configuration.Rec_bundle_802907493 {generated_oneof_descriptor_data as impl__Opts__generated_oneof_descriptor_data}
+*)
+include Sandwich_api_proto.Configuration.Rec_bundle_802907493 {t_Opts as t_Opts}
+(*)
+include Sandwich_api_proto.Configuration.Rec_bundle_802907493 {Opts_Client as Opts_Client}
+
+include Sandwich_api_proto.Configuration.Rec_bundle_802907493 {Opts_Server as Opts_Server}
+
+include Sandwich_api_proto.Configuration.Rec_bundle_802907493 {impl as impl}
+
+include Sandwich_api_proto.Configuration.Rec_bundle_802907493 {impl_1 as impl_1}
+*)
